\Large\textbf{Problem 1}

\begin{align*}
\sum_{x=0}^1 p(x|\mu) &= \sum_{x=0}^1 \mu^x(1-\mu)^{1-x}\\
&=\mu^0(1-\mu) + \mu(1-\mu)^0\\
&= 1-\mu + \mu\\
&= 1
\end{align*}

\begin{align*}
\Exp{x} &= \sum_{x=0}^1x\mu^x(1-\mu)^{1-x}\\
&= 0 + \mu(1-\mu)^0\\
&= \mu
\end{align*}

\begin{align*}
\var{x} &= \sum_{x=0}^1(x-\mu)^2\mu^x(1-\mu)^{1-x}\\
&= \mu^2(1-\mu) + (1-\mu)^2\mu\\
&= \mu^2-\mu^3 + (1-2\mu + \mu^2)\mu\\
&= \mu^2-\mu^3 + \mu-2\mu^2 + \mu^3\\
&= \mu-\mu^2\\
&= \mu(1-\mu)
\end{align*}

\begin{align*}
H[x] &= -\sum_{x=0}^1p(x)\ln p(x)\\
&= -\sum_{x=0}^1 \mu^x(1-\mu)^{1-x}\ln  \mu^x(1-\mu)^{1-x}\\
&= -(1-\mu)\ln (1-\mu)-\mu\ln\mu
\end{align*}

\Large\textbf{Problem 2}

\begin{align*}
\sum_{x\in \{-1,1\}} p(x|\mu) &= \sum_{x\in \{-1,1\}} \left(\frac{1 - \mu}{2}\right)^{(1-x)/2}\left(\frac{1 + \mu}{2}\right)^{(1+x)/2}\\
&=\left(\frac{1 - \mu}{2}\right) + \left(\frac{1 + \mu}{2}\right) \\
&= 1
\end{align*}

\begin{align*}
\Exp{x} &= \sum_{x\in \{-1,1\}} x\left(\frac{1 - \mu}{2}\right)^{(1-x)/2}\left(\frac{1 + \mu}{2}\right)^{(1+x)/2}\\
&= -\left(\frac{1 - \mu}{2}\right)+\left(\frac{1 + \mu}{2}\right)\\
&= \mu
\end{align*}

\begin{align*}
\var{x} &= \sum_{x\in \{-1,1\}} (x-\mu)^2\left(\frac{1 - \mu}{2}\right)^{(1-x)/2}\left(\frac{1 + \mu}{2}\right)^{(1+x)/2}\\
&= (-1-\mu)^2\left(\frac{1 - \mu}{2}\right)+(1-\mu)^2\left(\frac{1 + \mu}{2}\right)\\
&= \frac{(1+2\mu+\mu^2)(1-\mu) + (1-2\mu+\mu^2)(1+\mu)}{2}\\
&= 1- \mu^2
\end{align*}

\begin{align*}
H[x] &= -\sum_{x\in \{-1,1\}}p(x)\ln p(x)\\
&= -\sum_{x\in \{-1,1\}}\left(\frac{1 - \mu}{2}\right)^{\frac{1-x}{2}}\left(\frac{1 + \mu}{2}\right)^{\frac{1+x}{2}}\ln\left[\left(\frac{1 - \mu}{2}\right)^{\frac{1-x}{2}}\left(\frac{1 + \mu}{2}\right)^{\frac{1+x}{2}}\right]\\
&=-\left(\frac{1 - \mu}{2}\right)\ln \left(\frac{1 - \mu}{2}\right) - \left(\frac{1 + \mu}{2}\right)\ln \left(\frac{1 + \mu}{2}\right)\\
&= \frac{-(1-\mu)\ln(1-\mu) + (1-\mu)\ln(2) - (1+\mu)\ln(1+\mu) + (1+\mu)\ln(2)}{2}\\
\end{align*}

\Large\textbf{Problem 3}

First we prove that
\[{N\choose m} + {N \choose m-1} = {N+1 \choose m}\]

To show this imagine that we have  a box filled with $N$ blue balls and 1 red ball.  Then there are $N+1 \choose m$ different ways to draw balls from this box where order doesn't matter. We can break this up into two separate cases where we examine the number of ways to draw only blue balls from the box, and the number of ways to draw blue balls with a red ball. There are $N \choose m$ ways to draw only blue balls from the box because we remove the red ball from our selection so there are $N$ balls and we draw $m$ of them.  Then there are $N \choose m-1$ ways to draw balls from a box when we are gauranteed to have a red one in our selection.  This is because we select the red ball so we only have $N$ balls to choose the remaining blue from, and we only need to draw $m-1$ balls because we've already drawn the red.


Now to prove the binomial theorem we start with the base case where $N=0$.
\begin{align*}
(x+1)^m &= \sum_{m=0}^N {N \choose m}x^m\\
(x+1)^0 &= \sum_{m=0}^0 {0 \choose 0}x^0\\
1&=1
\end{align*}

Now we use the induction hypothesis to show that it is true for $N+1$
\begin{align*}
(x+1)^m &= \sum_{m=0}^N {N \choose m}x^m\\
(x+1)^m (x+1) &= (x+1)\sum_{m=0}^N {N \choose m}x^m\\
&= \sum_{m=0}^N {N \choose m}x^m + x\sum_{m=0}^N {N \choose m}x^m\\
&= \sum_{m=0}^N {N \choose m}x^m + \sum_{m=0}^N {N \choose m}x^{m+1}\\
&= \sum_{m=0}^N {N \choose m}x^m + \sum_{m=1}^{N+1} {N \choose m-1}x^{m+1 - 1}\\
&= {N \choose 0}x^0 + \sum_{m=1}^N \left[{N \choose m} + {N \choose m-1}\right]x^m + {N \choose N} x^{N+1}\\
&= {N \choose 0}x^0 + \sum_{m=1}^N {N + 1 \choose m}x^m + {N \choose N} x^{N+1}\\
&= \sum_{m=0}^N {N + 1 \choose m}x^m + {N \choose N} x^{N+1}\\
&= \sum_{m=0}^{N+1} {N + 1 \choose m}x^m\\
\end{align*}

Thus we have shown by induction that if our hypothesis is true for $N$ this implies that it is true for $N+1$ as well.

The last thing to show is that the binomial distribution is normalized.

\begin{align*}
\sum_{m=0}^N{N\choose m}\mu^m(1-\mu)^{N-m} &= (1-\mu)^N\sum_{m=0}^N{N\choose m}\mu^m(1-\mu)^{-m}\\
&= (1-\mu)^N\sum_{m=0}^N{N\choose m}\left(\frac{\mu}{1-\mu}\right)^m\\
&=(1-\mu)^N \left(1 + \frac{\mu}{1-\mu}\right)^N\\
&= \left(1 + \frac{\mu}{1-\mu} - \mu - \frac{\mu^2}{1-\mu}\right)^N\\
&=  \left(1 + \frac{\mu}{1-\mu} - \frac{\mu(1-\mu)}{1-\mu} - \frac{\mu^2}{1-\mu}\right)^N\\
&= \left(1 + \frac{\mu- \mu + \mu^2 - \mu^2}{1-\mu}\right)^N\\
&= 1^N\\
&= 1
\end{align*}


\Large\textbf{Problem 4}

To prove that the expected value of the binomial distribution is $N\mu$ we begin by differentiating both sides of the normalized distribution with respect to $\mu$ and then using basic algebra.

\begin{align*}
\sum_{m=0}^N{N\choose m}\mu^m(1-\mu)^{N-m} &= 1 \\
\frac{d}{d\mu}\sum_{m=0}^N{N\choose m}\mu^m(1-\mu)^{N-m} &= 0\\
\sum_{m=0}^N{N\choose m}m\mu^{m-1}(1-\mu)^{N-m}&= \sum_{m=0}^N(N-m){N\choose m}\mu^m(1-\mu)^{N-m-1}\\
(1-\mu)\sum_{m=0}^N{N\choose m}m\mu^{m-1}(1-\mu)^{N-m}&= \sum_{m=0}^N(N-m){N\choose m}\mu^m(1-\mu)^{N-m}\\
(1-\mu)\sum_{m=0}^N{N\choose m}m\mu^{m-1}(1-\mu)^{N-m}&= N - \Exp{m}\\
\sum_{m=0}^N{N\choose m}m\mu^{m-1}(1-\mu)^{N-m}&= N - \Exp{m} + \sum_{m=0}^N{N\choose m}m\mu^m(1-\mu)^{N-m}\\
\sum_{m=0}^N{N\choose m}m\mu^{m-1}(1-\mu)^{N-m}&= N - \Exp{m} + \Exp{m}\\
\mu\sum_{m=0}^N{N\choose m}m\mu^{m-1}(1-\mu)^{N-m}&= N\mu - \Exp{m}\\
\sum_{m=0}^N{N\choose m}m\mu^m(1-\mu)^{N-m}&= N\mu - \Exp{m}\\
\Exp{m} &= N\mu
\end{align*}

\newpage
\Large\textbf{Problem 6}

\begin{align*}
\Exp{x}&= \frac{\Gamma(a+b)}{\Gamma(a)\Gamma(b)}\int_0^1 x x^{\alpha -1}(1-x)^{\beta - 1}dx\\
&=   \frac{\Gamma(a+b)}{\Gamma(a)\Gamma(b)}\int_0^1 x^{\alpha}(1-x)^{\beta - 1}dx\\
&=  \frac{\Gamma(a+b)}{\Gamma(a)\Gamma(b)} \frac{\Gamma(a+1)\Gamma(b)}{\Gamma(a + b + 1)}\\
&=  \frac{\Gamma(a+b)}{\Gamma(a)} \frac{\Gamma(a+1)}{\Gamma(a + b + 1)}\\
&=  \frac{\Gamma(a+b)}{\Gamma(a)} \frac{a\Gamma(a)}{(a+b)\Gamma(a + b)}\\
&=  \frac{a}{a+b}\\
\end{align*}

To calculate the Variance I will use the fact that $\var{x} = \Exp{x^2} - \Exp{x}^2$  First let's calculate $\Exp{x^2}$

\begin{align*}
\Exp{x^2}&= \frac{\Gamma(a+b)}{\Gamma(a)\Gamma(b)}\int_0^1 x^2 x^{\alpha -1}(1-x)^{\beta - 1}dx\\
&= \frac{\Gamma(a+b)}{\Gamma(a)\Gamma(b)}\int_0^1 x^{\alpha + 1}(1-x)^{\beta - 1}dx\\
&=  \frac{\Gamma(a+b)}{\Gamma(a)\Gamma(b)}\frac{\Gamma(a+2)\Gamma(b)}{\Gamma(a + b + 2)}\\
&= \frac{\Gamma(a+b)}{\Gamma(a)}\frac{\Gamma(a+2)}{\Gamma(a + b + 2)}\\
&= \frac{\Gamma(a+b)}{\Gamma(a)}\frac{(a+1)a\Gamma(a)}{(a+b+1)(a+b)\Gamma(a + b)}\\
&= \frac{(a+1)a}{(a+b+1)(a+b)}\\
\end{align*}

Now we know that $\Exp{x}^2 = \left(\frac{a}{a+b}\right)^2$ so the Variance is:

\begin{align*}
\var{x} &= \Exp{x^2} - \Exp{x}^2\\
  &=  \frac{(a+1)a}{(a+b+1)(a+b)}- \frac{a^2}{(a + b)^2}\\
  &= \frac{(a+1)a(a+b) -  a^2(a + b + 1)}{(a+b+1)(a+b)^2}\\
  &= \frac{(a^2 + a)(a+b) -  (a^3 + a^2b + a^2)}{(a+b+1)(a+b)^2}\\
  &= \frac{a^3+a^2b+a^2+ab -  a^3 - a^2b - a^2}{(a+b+1)(a+b)^2}\\
  &= \frac{ab}{(a+b+1)(a+b)^2}\\
\end{align*}

Lastly the mode.  This can be calculated simply by taking the derivative of the Beta distribution and setting it equal to zero

\begin{align*}
\text{Beta}(\mu | a,b) &= \frac{\Gamma(a + b)}{\Gamma(a)\Gamma(b)}\mu^{a-1}(1-\mu)^{b-1}\\
0 &= \frac{d}{d\mu} \frac{\Gamma(a + b)}{\Gamma(a)\Gamma(b)}\mu^{a-1}(1-\mu)^{b-1}\\
&= \frac{d}{d\mu}\mu^{a-1}(1-\mu)^{b-1}\\
&= (a-1)\mu^{a-2}(1-\mu)^{b-1} -(b-1)\mu^{a-1}(1-\mu)^{b-2}\\
&= \mu^{a-2}(1-\mu)^{b-2}\left( (a-1)(1-\mu) -(b-1)\mu\right)\\
&= (a-1)(1-\mu) -(b-1)\mu\\
&= a-a\mu-1+\mu -b\mu+\mu\\
&= a-a\mu-1+\mu -b\mu+\mu\\
&= (a-1) - \mu(a + b - 2)\\
(1-a) &= -\mu(a + b -2)\\
\mu &= \frac{a - 1}{a + b - 2} 
\end{align*}

\Large\textbf{Problem 7}















