\subsection*{Problem 1}
This can be solved by substituting the definition of:
\begin{align*}
y(x, \mathbf{w}) &= \sum_{j=0}^Mw_jx^j
\end{align*}
into the error function and then taking the derivative.
\begin{align*}
  E(\mathbf{w}) &= \frac{1}{2} \sum_{n=1}^N\left(y(x, \w) - t_n\right)^2\\
  &= \frac{1}{2} \sum_{n=1}^N\left( \sum_{j=0}^Mw_jx^j - t_n\right)^2  && \text{Substitute}\\
  \frac{dE(\w)}{dw_i} &=  \sum_{n=1}^N\left(\left( \sum_{j=0}^Mw_jx^j - t_n\right)x^i \right)&& \text{Take the derivative}\\
  0 &= \sum_{n=1}^N\left(\left( \sum_{j=0}^Mw_jx^j - t_n\right)x^i\right) && \text{Set derivative to 0}\\
   0 &= \sum_{n=1}^N\left(\sum_{j=0}^Mw_jx^jx^i - t_nx^i\right) && \text{Set derivative to 0}\\
  \sum_{n=1}^N t_nx^i &=  \sum_{n=1}^N\sum_{j=0}^Mw_jx^jx^i\\
  \sum_{n=1}^N t_nx^i &=  \sum_{n=1}^N\sum_{j=0}^Mw_jx^{i+j}
  \end{align*}
  
 \subsection*{Problem 2}
 This is solved in almost the same way we just have one additional term for the regularization so:
 
 \begin{align*}
  E(\mathbf{w}) &= \frac{1}{2} \sum_{n=1}^N\left(y(x, \w) - t_n\right)^2 + \frac{\lambda}{2}\|\w\|^2\\
  &= \frac{1}{2} \sum_{n=1}^N\left( \sum_{j=0}^Mw_jx^j - t_n\right)^2  + \frac{\lambda}{2}\|\w\|^2\\\\
  \frac{dE(\w)}{dw_i} &=  \sum_{n=1}^N\left(\left( \sum_{j=0}^Mw_jx^j - t_n\right)x^i \right) + \lambda w_i\\\\
  -\lambda w_i &= \sum_{n=1}^N\left(\left( \sum_{j=0}^Mw_jx^j - t_n\right)x^i\right) + \lambda w_i \\
   -\lambda w_i &= \sum_{n=1}^N\left(\sum_{j=0}^Mw_jx^jx^i - t_nx^i\right) \\
  \sum_{n=1}^N t_nx^i - \lambda w_i&=  \sum_{n=1}^N\sum_{j=0}^Mw_jx^jx^i\\
  \sum_{n=1}^N t_nx^i -\lambda w_i&=  \sum_{n=1}^N\sum_{j=0}^Mw_jx^{i+j}
  \end{align*}
  
 
  



    
  